Communication_Topology_Analysis.thy
@@ -2,20 +2,99 @@ theory Communication_Topology_Analysis
   imports Main Syntax Semantics Abstract_Value_Flow_Analysis
 begin
 
-  
 
 datatype topo = OneShot | OneToOne | FanOut | FanIn | Any
+type_synonym topo_pair = "var \<times> topo"
+type_synonym topo_env = "var \<Rightarrow> topo"
+
+class com_topo =
+  fixes abstract_accept :: "abstract_value_env \<times> abstract_value_env \<Rightarrow> 'a \<Rightarrow> bool" (infix "\<Turnstile>" 55)
+  fixes exp_accept :: "exp \<Rightarrow> 'a \<Rightarrow> bool"
+  fixes path_accept :: "control_path \<Rightarrow> 'a \<Rightarrow> bool"
+
+definition (in com_topo) abstract_send_sites :: "var \<Rightarrow> 'a \<Rightarrow> var set" where
+  "abstract_send_sites x\<^sub>c e \<equiv> {x . \<exists> x\<^sub>e e' x\<^sub>m \<V> \<C>. 
+    exp_accept (LET x = SYNC x\<^sub>e in e') e \<and> 
+    abstract_accept (\<V>, \<C>) e \<and> 
+    {^Send_Evt x\<^sub>c x\<^sub>m} \<subseteq> \<V> x\<^sub>e
+  }"
+
+definition (in com_topo) abstract_recv_sites :: "var \<Rightarrow> 'a \<Rightarrow> var set" where
+  "abstract_recv_sites x\<^sub>c e \<equiv> {x . \<exists> x\<^sub>e e' \<V> \<C>. 
+    exp_accept (LET x = SYNC x\<^sub>e in e') e \<and> 
+    abstract_accept (\<V>, \<C>) e \<and> 
+    {^Recv_Evt x\<^sub>c} \<subseteq> \<V> x\<^sub>e
+  }"
+
+definition (in com_topo) control_paths :: "var set \<Rightarrow> 'a \<Rightarrow> control_path set" where 
+  "control_paths sites e \<equiv> {\<pi>;;x | \<pi> x . 
+    (x \<in> sites) \<and>  path_accept (\<pi>;;x) e
+  }" 
+
+definition (in com_topo) abstract_processes :: "var set \<Rightarrow> 'a \<Rightarrow> control_path set" where 
+  "abstract_processes sites e \<equiv> {\<pi> \<in> control_paths sites e .
+    (\<exists> \<pi>' . (\<pi> @ [Inr ()] @ \<pi>') \<in> control_paths sites e) \<or>
+    (\<forall> \<pi>' . (\<pi> @ \<pi>') \<notin> control_paths sites e)
+  }" 
+
+definition (in com_topo) abstract_send_paths :: "var \<Rightarrow> 'a \<Rightarrow> control_path set"  where 
+  "abstract_send_paths c e \<equiv> control_paths (abstract_send_sites c e) e"
+
+definition (in com_topo) abstract_recv_paths :: "var \<Rightarrow> 'a \<Rightarrow> control_path set"  where 
+  "abstract_recv_paths c e \<equiv> control_paths (abstract_recv_sites c e) e"
+
+definition (in com_topo) abstract_send_processes :: "var \<Rightarrow> 'a \<Rightarrow> control_path set"  where 
+  "abstract_send_processes c e = abstract_processes (abstract_send_sites c e) e"
+
+definition (in com_topo) abstract_recv_processes :: "var \<Rightarrow> 'a \<Rightarrow> control_path set"  where 
+  "abstract_recv_processes c e = abstract_processes (abstract_recv_sites c e) e"
+
+definition one_max :: "control_path set \<Rightarrow> bool"  where
+  "one_max \<T> \<equiv>  (\<nexists> p . p \<in> \<T>) \<or> (\<exists>! p . p \<in> \<T>)"
+
+
+inductive (in com_topo) topo_pair_accept :: "topo_pair \<Rightarrow> 'a \<Rightarrow> bool" (infix "\<TTurnstile>" 55) where
+  OneShot: "
+    one_max (abstract_send_paths c e) \<Longrightarrow> 
+    (c, OneShot) \<TTurnstile> e
+  " | 
+  OneToOne: "
+    \<lbrakk> 
+      one_max (abstract_send_processes c e) ;
+      one_max (abstract_recv_processes c e) 
+    \<rbrakk> \<Longrightarrow> 
+    (c, OneToOne) \<TTurnstile> e
+  " | 
+
+  FanOut: "
+    one_max (abstract_send_processes c e) \<Longrightarrow> 
+    (c, FanOut) \<TTurnstile> e
+  " | 
+
+  FanIn: "
+    one_max (abstract_recv_processes c e) \<Longrightarrow> 
+    (c, FanIn) \<TTurnstile> e
+  " | 
+
+  Any: "(c, Any) \<TTurnstile> e"
+
+
+
+
+(***************)
+
+
 
 definition send_sites :: "state_pool \<Rightarrow> chan \<Rightarrow> control_path set" where
   "send_sites \<E> ch = {\<pi>. \<exists> x x\<^sub>e e \<kappa> \<rho> x\<^sub>c x\<^sub>m \<rho>\<^sub>e. 
-    \<E> \<pi> = Some (<<LET x = SYNC x\<^sub>e in e, \<rho>, \<kappa>>>) \<and> 
+    \<E> \<pi> = Some (\<langle>LET x = SYNC x\<^sub>e in e; \<rho>; \<kappa>\<rangle>) \<and> 
     \<rho> x\<^sub>e = Some \<lbrace>Send_Evt x\<^sub>c x\<^sub>m, \<rho>\<^sub>e\<rbrace> \<and> 
     \<rho>\<^sub>e x\<^sub>c = Some \<lbrace>ch\<rbrace>
   }"
 
 definition recv_sites :: "state_pool \<Rightarrow> chan \<Rightarrow> control_path set" where
   "recv_sites \<E> ch = {\<pi>. \<exists> x x\<^sub>e e \<kappa> \<rho> x\<^sub>c \<rho>\<^sub>e. 
-    \<E> \<pi> = Some (<<LET x = SYNC x\<^sub>e in e, \<rho>, \<kappa>>>) \<and> 
+    \<E> \<pi> = Some (\<langle>LET x = SYNC x\<^sub>e in e; \<rho>; \<kappa>\<rangle>) \<and> 
     \<rho> x\<^sub>e = Some \<lbrace>Recv_Evt x\<^sub>c, \<rho>\<^sub>e\<rbrace> \<and> 
     \<rho>\<^sub>e x\<^sub>c = Some \<lbrace>ch\<rbrace>
   }"
@@ -29,7 +108,6 @@ definition single_side :: "(state_pool \<Rightarrow> chan \<Rightarrow> control_
 
 definition one_shot :: "state_pool \<Rightarrow> chan \<Rightarrow> bool" where
   "one_shot \<E> c \<longleftrightarrow> card (send_sites \<E> c) \<le> 1"
-
 
 definition single_receiver :: "state_pool \<Rightarrow> chan \<Rightarrow> bool" where 
   "single_receiver = single_side recv_sites"
@@ -47,11 +125,7 @@ definition fan_in :: "state_pool \<Rightarrow> chan \<Rightarrow> bool" where
   "fan_in \<E> c \<longleftrightarrow> \<not> single_sender \<E> c \<and> single_receiver \<E> c"
 
 definition var_topo :: "(state_pool \<Rightarrow> chan \<Rightarrow> bool) \<Rightarrow> state_pool \<Rightarrow> var \<Rightarrow> bool" where
-  "var_topo t \<E> x \<longleftrightarrow> (\<forall> \<pi> . \<exists> x' e' \<rho>' \<kappa>' . \<E> \<pi> = Some (<<LET x' = CHAN \<lparr>\<rparr> in e', \<rho>', \<kappa>'>>) \<longrightarrow> t \<E> (Ch \<pi> x))"
-
-type_synonym topo_pair = "var \<times> topo"
-
-type_synonym topo_env = "var \<Rightarrow> topo"
+  "var_topo t \<E> x \<longleftrightarrow> (\<forall> \<pi> . \<exists> x' e' \<rho>' \<kappa>' . \<E> \<pi> = Some (\<langle>LET x' = CHAN \<lparr>\<rparr> in e'; \<rho>'; \<kappa>'\<rangle>) \<longrightarrow> t \<E> (Ch \<pi> x))"
 
 definition var_to_topo :: "state_pool \<Rightarrow> var \<Rightarrow> topo" ("\<langle>\<langle>_ ; _\<rangle>\<rangle>" [0,0]61) where
   "\<langle>\<langle>\<E> ; x\<rangle>\<rangle> = 
@@ -62,11 +136,8 @@ definition var_to_topo :: "state_pool \<Rightarrow> var \<Rightarrow> topo" ("\<
     else Any))))
   "
 
-
-
 definition state_pool_to_topo_env :: "state_pool \<Rightarrow> topo_env" ("\<langle>\<langle>_\<rangle>\<rangle>" [0]61) where
   "\<langle>\<langle>\<E>\<rangle>\<rangle> = (\<lambda> x . \<langle>\<langle>\<E> ; x\<rangle>\<rangle>)"
-
 
 inductive precision_order :: "topo \<Rightarrow> topo \<Rightarrow> bool" (infix "\<preceq>" 55) where  
   Edge1 : "OneShot \<preceq> OneToOne" | 
@@ -139,153 +210,41 @@ inductive path_in_exp' :: "abstract_value_env \<Rightarrow> control_path \<Right
   " 
 
 definition path_in_exp :: "control_path \<Rightarrow> exp \<Rightarrow> bool" (infix "\<triangleleft>" 55)where
-  "\<pi> \<triangleleft> e \<equiv> (\<exists> \<V> \<C> . (\<V>, \<C>) \<Turnstile> e \<and> (\<V> \<Turnstile> \<pi> \<triangleleft> e))"
+  "\<pi> \<triangleleft> e \<equiv> (\<exists> \<V> \<C> . (\<V>, \<C>) \<Turnstile>\<^sub>e e \<and> (\<V> \<Turnstile> \<pi> \<triangleleft> e))"
 
 inductive subexp :: "exp \<Rightarrow> exp \<Rightarrow> bool" (infix "\<unlhd>" 55)where
   Refl: "e \<unlhd> e" |
   Step: "e' \<unlhd> e \<Longrightarrow> e' \<unlhd> (LET x = b in e)"
 
-
-class xyz =
-  fixes accept :: "abstract_value_env \<times> abstract_value_env \<Rightarrow> 'a \<Rightarrow> bool"
-  fixes exp_in :: "exp \<Rightarrow> 'a \<Rightarrow> bool"
-  fixes path_in :: "control_path \<Rightarrow> 'a \<Rightarrow> bool"
-
-
-definition (in xyz) abstract_send_sites :: "var \<Rightarrow> 'a \<Rightarrow> var set" where
-  "abstract_send_sites x\<^sub>c e = {x . \<exists> x\<^sub>e e' x\<^sub>m \<V> \<C>. 
-    exp_in (LET x = SYNC x\<^sub>e in e') e \<and> 
-    accept (\<V>, \<C>) e \<and> 
-    {^Send_Evt x\<^sub>c x\<^sub>m} \<subseteq> \<V> x\<^sub>e
-  }"
-
-definition (in xyz) abstract_recv_sites :: "var \<Rightarrow> 'a \<Rightarrow> var set" where
-  "abstract_recv_sites x\<^sub>c e = {x . \<exists> x\<^sub>e e' \<V> \<C>. 
-    exp_in (LET x = SYNC x\<^sub>e in e') e \<and> 
-    accept (\<V>, \<C>) e \<and> 
-    {^Recv_Evt x\<^sub>c} \<subseteq> \<V> x\<^sub>e
-  }"
-
-instantiation exp :: xyz
+instantiation exp :: com_topo
 begin
-definition accept_exp: "accept \<T> e = flow_accept \<T> e" 
-definition exp_in_exp: "exp_in e' e = subexp e' e" 
-definition path_in_exp: "path_in \<pi> e = \<pi> \<triangleleft> e" 
-instance proof
-qed
-end
+definition abstract_accept_exp where "\<T> \<Turnstile> e \<equiv> \<T> \<Turnstile>\<^sub>e e" 
+definition exp_accept_exp where "exp_accept e' e \<equiv> e' \<unlhd> e"
+definition path_accept_exp where "path_accept \<pi> e \<equiv> \<pi> \<triangleleft> e"
+instance proof qed
+end 
 
-definition (in xyz) control_paths :: "var set \<Rightarrow> 'a \<Rightarrow> control_path set" where 
-  "control_paths sites e = {\<pi>;;x | \<pi> x . 
-    (x \<in> sites) \<and>  path_in (\<pi>;;x) e
-  }" 
-
-definition (in xyz) abstract_processes :: "var set \<Rightarrow> 'a \<Rightarrow> control_path set" where 
-  "abstract_processes sites e = {\<pi> \<in> control_paths sites e .
-    (\<exists> \<pi>' . (\<pi> @ [Inr ()] @ \<pi>') \<in> control_paths sites e) \<or>
-    (\<forall> \<pi>' . (\<pi> @ \<pi>') \<notin> control_paths sites e)
-  }" 
-
-definition (in xyz) abstract_send_paths :: "var \<Rightarrow> 'a \<Rightarrow> control_path set"  where 
-  "abstract_send_paths c e = control_paths (abstract_send_sites c e) e"
-
-definition (in xyz) abstract_recv_paths :: "var \<Rightarrow> 'a \<Rightarrow> control_path set"  where 
-  "abstract_recv_paths c e = control_paths (abstract_recv_sites c e) e"
-
-definition (in xyz) abstract_send_processes :: "var \<Rightarrow> 'a \<Rightarrow> control_path set"  where 
-  "abstract_send_processes c e = abstract_processes (abstract_send_sites c e) e"
-
-definition (in xyz) abstract_recv_processes :: "var \<Rightarrow> 'a \<Rightarrow> control_path set"  where 
-  "abstract_recv_processes c e = abstract_processes (abstract_recv_sites c e) e"
-
-definition one_max :: "control_path set \<Rightarrow> bool"  where
-  "one_max \<T> \<equiv>  (\<nexists> p . p \<in> \<T>) \<or> (\<exists>! p . p \<in> \<T>)"
-
-
-inductive (in xyz) topo_pair_accept :: "topo_pair \<Rightarrow> 'a \<Rightarrow> bool" (infix "\<Turnstile>\<^sub>t" 55) where
-  OneShot: "
-    one_max (abstract_send_paths c e) \<Longrightarrow> 
-    (c, OneShot) \<Turnstile>\<^sub>t e
-  " | 
-  OneToOne: "
-    \<lbrakk> 
-      one_max (abstract_send_processes c e) ;
-      one_max (abstract_recv_processes c e) 
-    \<rbrakk> \<Longrightarrow> 
-    (c, OneToOne) \<Turnstile>\<^sub>t e
-  " | 
-
-  FanOut: "
-    one_max (abstract_send_processes c e) \<Longrightarrow> 
-    (c, FanOut) \<Turnstile>\<^sub>t e
-  " | 
-
-  FanIn: "
-    one_max (abstract_recv_processes c e) \<Longrightarrow> 
-    (c, FanIn) \<Turnstile>\<^sub>t e
-  " | 
-
-  Any: "(c, Any) \<Turnstile>\<^sub>t e"
 
 definition topo_accept :: "topo_env \<Rightarrow> exp \<Rightarrow> bool" (infix "\<bind>" 55) where 
-  "\<A> \<bind> e \<longleftrightarrow> (\<forall> x . (x, \<A> x) \<Turnstile>\<^sub>t e)"
-
-
-
+  "\<A> \<bind> e \<equiv> (\<forall> x . (x, \<A> x) \<TTurnstile> e)"
 
 
 inductive exp_in_pool :: "exp \<Rightarrow> state_pool \<Rightarrow> bool" (infix "\<lhd>|" 55)where
   Any: "
     \<lbrakk>
-      \<E> \<pi> = Some (<<e, \<rho>, \<kappa>>>);
+      \<E> \<pi> = Some (\<langle>e; \<rho>; \<kappa>\<rangle>);
       e' \<unlhd> e
     \<rbrakk> \<Longrightarrow>
     e' \<lhd>| \<E>
   "
 
-
-definition abstract_send_sites_pool :: "var \<Rightarrow> state_pool \<Rightarrow> var set" where
-  "abstract_send_sites_pool x\<^sub>c \<E> = {x . \<exists> x\<^sub>e e' x\<^sub>m \<V> \<C>. 
-    (LET x = SYNC x\<^sub>e in e') \<lhd>| \<E> \<and> 
-    (\<V>, \<C>) \<parallel>\<lless> \<E> \<and> 
-    {^Send_Evt x\<^sub>c x\<^sub>m} \<subseteq> \<V> x\<^sub>e
-  }"
-
-definition abstract_recv_sites_pool :: "var \<Rightarrow> state_pool \<Rightarrow> var set" where
-  "abstract_recv_sites_pool x\<^sub>c \<E> = {x . \<exists> x\<^sub>e e' \<V> \<C>. 
-    (LET x = SYNC x\<^sub>e in e') \<lhd>| \<E> \<and> 
-    (\<V>, \<C>) \<parallel>\<lless> \<E> \<and> 
-    {^Recv_Evt x\<^sub>c} \<subseteq> \<V> x\<^sub>e
-  }"
-
-
-
-inductive topo_pair_over_pool_accept :: "topo_pair \<Rightarrow> state_pool \<Rightarrow> bool" (infix "\<parallel>\<lless>\<^sub>t" 55) where
-  Any: "
-    (\<forall> \<pi> \<sigma> . \<E> \<pi> = Some \<sigma> \<longrightarrow> (x, t) \<TTurnstile>\<^sub>t \<sigma>)
-    \<Longrightarrow> 
-    (x, t) \<parallel>\<lless>\<^sub>t \<E>
-  "
-
-(*
-
-inductive topo_pair_over_value_accept :: "topo_pair \<Rightarrow> val \<Rightarrow> bool" (infix "\<parallel>>\<^sub>t" 55)
-and  topo_pair_over_env_accept :: "topo_pair \<Rightarrow> (var \<rightharpoonup> val) \<Rightarrow> bool" (infix "\<parallel>\<approx>\<^sub>t" 55) 
-where
-inductive topo_pair_over_stack_accept :: "topo_pair \<Rightarrow> cont list \<Rightarrow> bool" ("_ \<Turnstile>\<^sub>t _ \<Rrightarrow> _" [56, 0, 56] 55)
-
-inductive topo_pair_over_state_accept :: "topo_pair \<Rightarrow> state \<Rightarrow> bool" (infix "\<TTurnstile>\<^sub>t" 55) where
-  Any: "
-    \<lbrakk>
-      (\<V>, \<C>) \<Turnstile> e; 
-      (\<V>, \<C>) \<parallel>\<approx> \<rho>; 
-      (\<V>, \<C>) \<Turnstile> \<V> (\<lfloor>e\<rfloor>) \<Rrightarrow> \<kappa>
-    \<rbrakk> \<Longrightarrow>
-    (\<V>, \<C>) \<TTurnstile> <<e, \<rho>, \<kappa>>>
-  "
-
-
-*)
- 
+datatype state_pool' = SP state_pool
+instantiation state_pool' :: com_topo
+begin
+fun abstract_accept_state_pool' where "\<T> \<Turnstile> (SP \<E>) = \<T> \<Turnstile>\<^sub>\<E> \<E>" 
+fun exp_accept_state_pool' where "exp_accept e' (SP \<E>) = e' \<lhd>| \<E>"
+fun path_accept_state_pool' where "path_accept \<pi> (SP \<E>) = \<pi> \<triangleleft> e"
+instance proof qed
+end 
 
 end
