Semantics.thy
@@ -9,103 +9,67 @@ datatype chan = Ch control_path var
 
 datatype val = 
   V_Chan chan ("\<lbrace>_\<rbrace>") |
-  V_Closure prim env ("\<lbrace>_, _\<rbrace>") |
+  V_Closure prim "var \<rightharpoonup> val" ("\<lbrace>_, _\<rbrace>") |
   V_Unit ("\<lbrace>\<rbrace>")
-and env = Env "var \<rightharpoonup> val"
+ 
+type_synonym val_env = "var \<rightharpoonup> val"
 
-inductive env_entry_accept :: "env \<Rightarrow> var \<Rightarrow> val \<Rightarrow> bool" ("_ _ \<rhd> _" [56, 0, 56]55)where
-  Any: "
-    (f x = Some \<omega>)
-    \<Longrightarrow> 
-    (Env f) x \<rhd> \<omega>
-  "
+datatype cont = Cont var exp val_env ("\<langle>_,_,_\<rangle>" [0, 0, 0] 70) 
 
-
-fun env_update :: "env \<Rightarrow> (var \<rightharpoonup> val) \<Rightarrow> env" (infixl "@:" 61) where
-  "(Env f) @: mp = Env (f ++ mp)" 
-
-
-datatype cont = Cont var exp env ("\<langle>_,_,_\<rangle>" [0, 0, 0] 70) 
-
-datatype cont_stack = CS "cont list"
-
-abbreviation empty_cont_stack :: "cont_stack" ("[.]" 71) where
-  "empty_cont_stack \<equiv> CS []"
-
-fun cont_stack_cons :: "cont \<Rightarrow> cont_stack \<Rightarrow> cont_stack" (infix ":#" 61) where
-  "c :# (CS l) = CS (c # l)"
-
-datatype state = State exp env cont_stack ("\<langle>_;_;_\<rangle>" [0, 0, 0] 71) 
+datatype state = State exp val_env "cont list" ("\<langle>_;_;_\<rangle>" [0, 0, 0] 71) 
   
-datatype state_pool = SP "control_path \<rightharpoonup> state"
-
-inductive state_pool_entry_accept :: "state_pool \<Rightarrow> control_path \<Rightarrow> state \<Rightarrow> bool" ("_ _ \<diamond> _" [56, 0, 56]55)where
-  Any: "
-    (f \<pi> = Some \<omega>)
-    \<Longrightarrow> 
-    (SP f) x \<diamond> \<omega>
-  "
-
-inductive state_pool_none_accept :: "state_pool \<Rightarrow> control_path \<Rightarrow> bool" ("_ _ \<diamond>." [56, 0]55)where
-  Any: "
-    (f \<pi> = None)
-    \<Longrightarrow> 
-    (SP f) \<pi> \<diamond>.
-  "
-
-fun state_pool_update :: "state_pool \<Rightarrow> (control_path \<rightharpoonup> state) \<Rightarrow> state_pool" (infixl "+:" 61) where
-  "(SP f) +: mp = SP (f ++ mp)"
+type_synonym state_pool = "control_path \<rightharpoonup> state"
 
   
 inductive seq_step :: "state \<Rightarrow> state \<Rightarrow> bool" (infix "\<hookrightarrow>" 55) where 
   Result: "
-    \<rho> x \<rhd> \<omega> \<Longrightarrow>
-    \<langle>RESULT x; \<rho>; \<langle>x\<^sub>\<kappa>, e\<^sub>\<kappa>, \<rho>\<^sub>\<kappa>\<rangle> :# \<kappa>\<rangle>\<hookrightarrow> \<langle>e\<^sub>\<kappa>; \<rho>\<^sub>\<kappa> @: [x\<^sub>\<kappa> \<mapsto> \<omega>]; \<kappa>\<rangle>
+    \<rho> x = Some \<omega> \<Longrightarrow>
+    \<langle>RESULT x; \<rho>; \<langle>x\<^sub>\<kappa>, e\<^sub>\<kappa>, \<rho>\<^sub>\<kappa>\<rangle> # \<kappa>\<rangle>\<hookrightarrow> \<langle>e\<^sub>\<kappa>; \<rho>\<^sub>\<kappa> ++ [x\<^sub>\<kappa> \<mapsto> \<omega>]; \<kappa>\<rangle>
   " |
   Let_Unit: "
-    \<langle>LET x = \<lparr>\<rparr> in e; \<rho>; \<kappa>\<rangle> \<hookrightarrow> \<langle>e; \<rho> @: [x \<mapsto> \<lbrace>\<rbrace>]; \<kappa>\<rangle>
+    \<langle>LET x = \<lparr>\<rparr> in e; \<rho>; \<kappa>\<rangle> \<hookrightarrow> \<langle>e; \<rho> ++ [x \<mapsto> \<lbrace>\<rbrace>]; \<kappa>\<rangle>
   " |
   Let_Prim: "
-    \<langle>LET x = Prim p in e; \<rho>; \<kappa>\<rangle> \<hookrightarrow> \<langle>e; \<rho> @: [x \<mapsto> \<lbrace>p, \<rho>\<rbrace>]; \<kappa>\<rangle>
+    \<langle>LET x = Prim p in e; \<rho>; \<kappa>\<rangle> \<hookrightarrow> \<langle>e; \<rho> ++ [x \<mapsto> \<lbrace>p, \<rho>\<rbrace>]; \<kappa>\<rangle>
   " |
   Let_Case_Left: "
     \<lbrakk>
-      \<rho> x\<^sub>s \<rhd> \<lbrace>Left x\<^sub>l', \<rho>\<^sub>l\<rbrace>; 
-      \<rho>\<^sub>l x\<^sub>l' \<rhd> \<omega>\<^sub>l 
+      \<rho> x\<^sub>s = Some \<lbrace>Left x\<^sub>l', \<rho>\<^sub>l\<rbrace>; 
+      \<rho>\<^sub>l x\<^sub>l' = Some \<omega>\<^sub>l 
     \<rbrakk> \<Longrightarrow>
-    \<langle>LET x = CASE x\<^sub>s LEFT x\<^sub>l |> e\<^sub>l RIGHT x\<^sub>r |> e\<^sub>r in e; \<rho>; \<kappa>\<rangle> \<hookrightarrow> \<langle>e\<^sub>l; \<rho> @: [x\<^sub>l \<mapsto> \<omega>\<^sub>l]; \<langle>x, e, \<rho>\<rangle> :# \<kappa>\<rangle>
+    \<langle>LET x = CASE x\<^sub>s LEFT x\<^sub>l |> e\<^sub>l RIGHT x\<^sub>r |> e\<^sub>r in e; \<rho>; \<kappa>\<rangle> \<hookrightarrow> \<langle>e\<^sub>l; \<rho> ++ [x\<^sub>l \<mapsto> \<omega>\<^sub>l]; \<langle>x, e, \<rho>\<rangle> # \<kappa>\<rangle>
   " |
   Let_Case_Right: "
     \<lbrakk>
-      \<rho> x\<^sub>s \<rhd> \<lbrace>Right x\<^sub>r', \<rho>\<^sub>r\<rbrace>; 
-      \<rho>\<^sub>r x\<^sub>r' \<rhd> \<omega>\<^sub>r 
+      \<rho> x\<^sub>s = Some \<lbrace>Right x\<^sub>r', \<rho>\<^sub>r\<rbrace>; 
+      \<rho>\<^sub>r x\<^sub>r' = Some \<omega>\<^sub>r 
     \<rbrakk> \<Longrightarrow>
-    \<langle>LET x = CASE x\<^sub>s LEFT x\<^sub>l |> e\<^sub>l RIGHT x\<^sub>r |> e\<^sub>r in e; \<rho>; \<kappa>\<rangle> \<hookrightarrow> \<langle>e\<^sub>r; \<rho> @: [x\<^sub>r \<mapsto> \<omega>\<^sub>r]; \<langle>x, e, \<rho>\<rangle> :# \<kappa>\<rangle>
+    \<langle>LET x = CASE x\<^sub>s LEFT x\<^sub>l |> e\<^sub>l RIGHT x\<^sub>r |> e\<^sub>r in e; \<rho>; \<kappa>\<rangle> \<hookrightarrow> \<langle>e\<^sub>r; \<rho> ++ [x\<^sub>r \<mapsto> \<omega>\<^sub>r]; \<langle>x, e, \<rho>\<rangle> # \<kappa>\<rangle>
   " |
   Fst: "
     \<lbrakk> 
-      \<rho> x\<^sub>p \<rhd> \<lbrace>Pair x\<^sub>1 x\<^sub>2, \<rho>\<^sub>p\<rbrace>; 
-      \<rho>\<^sub>p x\<^sub>1 \<rhd> \<omega> 
+      \<rho> x\<^sub>p = Some \<lbrace>Pair x\<^sub>1 x\<^sub>2, \<rho>\<^sub>p\<rbrace>; 
+      \<rho>\<^sub>p x\<^sub>1 = Some \<omega> 
     \<rbrakk> \<Longrightarrow>
-    \<langle>LET x = FST x\<^sub>p in e; \<rho>; \<kappa>\<rangle> \<hookrightarrow> \<langle>e; \<rho> @: [x \<mapsto> \<omega>]; \<kappa>\<rangle>
+    \<langle>LET x = FST x\<^sub>p in e; \<rho>; \<kappa>\<rangle> \<hookrightarrow> \<langle>e; \<rho> ++ [x \<mapsto> \<omega>]; \<kappa>\<rangle>
   " |
   Snd: "
     \<lbrakk> 
-      \<rho> x\<^sub>p \<rhd> \<lbrace>Pair x\<^sub>1 x\<^sub>2, \<rho>\<^sub>p\<rbrace>; 
-      \<rho>\<^sub>p x\<^sub>2 \<rhd> \<omega> 
+      \<rho> x\<^sub>p = Some \<lbrace>Pair x\<^sub>1 x\<^sub>2, \<rho>\<^sub>p\<rbrace>; 
+      \<rho>\<^sub>p x\<^sub>2 = Some \<omega> 
     \<rbrakk> \<Longrightarrow>
-    \<langle>LET x = SND x\<^sub>p in e; \<rho>; \<kappa>\<rangle> \<hookrightarrow> \<langle>e; \<rho> @: [x \<mapsto> \<omega>]; \<kappa>\<rangle>
+    \<langle>LET x = SND x\<^sub>p in e; \<rho>; \<kappa>\<rangle> \<hookrightarrow> \<langle>e; \<rho> ++ [x \<mapsto> \<omega>]; \<kappa>\<rangle>
   " |
   Let_App: "
     \<lbrakk>
-      \<rho> f \<rhd> \<lbrace>Abs f\<^sub>l x\<^sub>l e\<^sub>l, \<rho>\<^sub>l\<rbrace> ; 
-      \<rho> x\<^sub>a \<rhd> \<omega>\<^sub>a 
+      \<rho> f = Some \<lbrace>Abs f\<^sub>l x\<^sub>l e\<^sub>l, \<rho>\<^sub>l\<rbrace> ; 
+      \<rho> x\<^sub>a = Some \<omega>\<^sub>a 
     \<rbrakk> \<Longrightarrow>
     \<langle>LET x = APP f x\<^sub>a in e; \<rho>; \<kappa>\<rangle> \<hookrightarrow> 
-    \<langle>e\<^sub>l; \<rho>\<^sub>l @: [f\<^sub>l \<mapsto> \<lbrace>Abs f\<^sub>l x\<^sub>l e\<^sub>l, \<rho>\<^sub>l\<rbrace>, x\<^sub>l \<mapsto> \<omega>\<^sub>a]; \<langle>x, e, \<rho>\<rangle> :# \<kappa>\<rangle>
+    \<langle>e\<^sub>l; \<rho>\<^sub>l ++ [f\<^sub>l \<mapsto> \<lbrace>Abs f\<^sub>l x\<^sub>l e\<^sub>l, \<rho>\<^sub>l\<rbrace>, x\<^sub>l \<mapsto> \<omega>\<^sub>a]; \<langle>x, e, \<rho>\<rangle> # \<kappa>\<rangle>
   "
 
-inductive_cases Result_E[elim!]: "\<langle>RESULT x; \<rho>; \<langle>x\<^sub>\<kappa>, e\<^sub>\<kappa>, \<rho>\<^sub>\<kappa>\<rangle> :# \<kappa>\<rangle> \<hookrightarrow> \<langle>e\<^sub>\<kappa>; \<rho>\<^sub>\<kappa> @: [x\<^sub>\<kappa> \<mapsto> \<omega>]; \<kappa>\<rangle>"
+inductive_cases Result_E[elim!]: "\<langle>RESULT x; \<rho>; \<langle>x\<^sub>\<kappa>, e\<^sub>\<kappa>, \<rho>\<^sub>\<kappa>\<rangle> # \<kappa>\<rangle> \<hookrightarrow> \<langle>e\<^sub>\<kappa>; \<rho>\<^sub>\<kappa> ++ [x\<^sub>\<kappa> \<mapsto> \<omega>]; \<kappa>\<rangle>"
 
 abbreviation control_path_append_var :: "control_path => var => control_path" (infixl ";;" 61) where
   "\<pi>;;x \<equiv> \<pi> @ [Inl x]"
@@ -115,12 +79,12 @@ abbreviation control_path_append_unit :: "control_path  => control_path" ("_;;."
   
   
 definition leaf :: "state_pool \<Rightarrow> control_path \<Rightarrow> bool" where
-  "leaf \<E> \<pi> \<equiv> \<not>(\<E> \<pi> \<diamond>.) \<and> (\<nexists> \<pi>' . \<not>(\<E> \<pi>' \<diamond>.) \<and> strict_prefix \<pi> \<pi>')"
+  "leaf \<E> \<pi> \<equiv> \<not>(\<E> \<pi> = None) \<and> (\<nexists> \<pi>' . \<not>(\<E> \<pi>' = None) \<and> strict_prefix \<pi> \<pi>')"
 
 
 lemma leaf_elim: "
   \<lbrakk> leaf \<E> \<pi>; strict_prefix \<pi> \<pi>' \<rbrakk> \<Longrightarrow>
-   \<E> \<pi>' \<diamond>.
+   \<E> \<pi>' = None
 "
 using leaf_def by blast
 (*
@@ -209,53 +173,53 @@ inductive concur_step :: "state_pool \<Rightarrow> state_pool \<Rightarrow> bool
   Seq_Step: "
     \<lbrakk> 
       leaf \<E> \<pi> ;
-      \<E> \<pi> \<diamond> \<langle>LET x = b in e'; \<rho>; \<kappa>\<rangle> ;
+      \<E> \<pi> = Some (\<langle>LET x = b in e; \<rho>; \<kappa>\<rangle>) ;
       \<langle>LET x = b in e; \<rho>; \<kappa>\<rangle> \<hookrightarrow> \<sigma>'
     \<rbrakk> \<Longrightarrow>
-    \<E> \<rightarrow> \<E> +: [\<pi>;;x \<mapsto> \<sigma>']
+    \<E> \<rightarrow> \<E> ++ [\<pi>;;x \<mapsto> \<sigma>']
   " |
   Sync: "
     \<lbrakk>
    
       leaf \<E> \<pi>\<^sub>s ;
-      \<E> \<pi>\<^sub>s \<diamond> \<langle>LET x\<^sub>s = SYNC x\<^sub>s\<^sub>e in e\<^sub>s; \<rho>\<^sub>s; \<kappa>\<^sub>s\<rangle>;
-      \<rho>\<^sub>s x\<^sub>s\<^sub>e \<rhd> \<lbrace>Send_Evt x\<^sub>s\<^sub>c x\<^sub>m, \<rho>\<^sub>s\<^sub>e\<rbrace>;
-      \<rho>\<^sub>s\<^sub>e x\<^sub>s\<^sub>c \<rhd> \<lbrace>c\<rbrace>; 
+      \<E> \<pi>\<^sub>s = Some (\<langle>LET x\<^sub>s = SYNC x\<^sub>s\<^sub>e in e\<^sub>s; \<rho>\<^sub>s; \<kappa>\<^sub>s\<rangle>);
+      \<rho>\<^sub>s x\<^sub>s\<^sub>e = Some \<lbrace>Send_Evt x\<^sub>s\<^sub>c x\<^sub>m, \<rho>\<^sub>s\<^sub>e\<rbrace>;
+      \<rho>\<^sub>s\<^sub>e x\<^sub>s\<^sub>c = Some \<lbrace>c\<rbrace>; 
       
-      \<rho>\<^sub>s\<^sub>e x\<^sub>m \<rhd> \<omega>\<^sub>m ;
+      \<rho>\<^sub>s\<^sub>e x\<^sub>m = Some \<omega>\<^sub>m ;
 
       leaf \<E> \<pi>\<^sub>r ;
-      \<E> \<pi>\<^sub>r \<diamond> \<langle>LET x\<^sub>r = SYNC x\<^sub>r\<^sub>e in e\<^sub>r; \<rho>\<^sub>r; \<kappa>\<^sub>r\<rangle>;
-      \<rho>\<^sub>r x\<^sub>r\<^sub>e \<rhd> \<lbrace>Recv_Evt x\<^sub>r\<^sub>c, \<rho>\<^sub>r\<^sub>e\<rbrace>;
-      \<rho>\<^sub>r\<^sub>e x\<^sub>r\<^sub>c \<rhd> \<lbrace>c\<rbrace>
+      \<E> \<pi>\<^sub>r = Some (\<langle>LET x\<^sub>r = SYNC x\<^sub>r\<^sub>e in e\<^sub>r; \<rho>\<^sub>r; \<kappa>\<^sub>r\<rangle>);
+      \<rho>\<^sub>r x\<^sub>r\<^sub>e = Some \<lbrace>Recv_Evt x\<^sub>r\<^sub>c, \<rho>\<^sub>r\<^sub>e\<rbrace>;
+      \<rho>\<^sub>r\<^sub>e x\<^sub>r\<^sub>c = Some \<lbrace>c\<rbrace>
 
     \<rbrakk> \<Longrightarrow>
-    \<E> \<rightarrow> \<E> +: [
-      \<pi>\<^sub>s;;x\<^sub>s \<mapsto> (\<langle>e\<^sub>s; \<rho>\<^sub>s @: [x\<^sub>s \<mapsto> \<lbrace>\<rbrace>]; \<kappa>\<^sub>s\<rangle>), 
-      \<pi>\<^sub>r;;x\<^sub>r \<mapsto> (\<langle>e\<^sub>r; \<rho>\<^sub>r @: [x\<^sub>r \<mapsto> \<omega>\<^sub>m]; \<kappa>\<^sub>r\<rangle>)
+    \<E> \<rightarrow> \<E> ++ [
+      \<pi>\<^sub>s;;x\<^sub>s \<mapsto> (\<langle>e\<^sub>s; \<rho>\<^sub>s ++ [x\<^sub>s \<mapsto> \<lbrace>\<rbrace>]; \<kappa>\<^sub>s\<rangle>), 
+      \<pi>\<^sub>r;;x\<^sub>r \<mapsto> (\<langle>e\<^sub>r; \<rho>\<^sub>r ++ [x\<^sub>r \<mapsto> \<omega>\<^sub>m]; \<kappa>\<^sub>r\<rangle>)
     ]
   " |
   Let_Chan: "
     \<lbrakk> 
       leaf \<E> \<pi> ;
-      \<E> \<pi> \<diamond> \<langle>LET x = CHAN \<lparr>\<rparr> in e; \<rho>; \<kappa>\<rangle>
+      \<E> \<pi> = Some (\<langle>LET x = CHAN \<lparr>\<rparr> in e; \<rho>; \<kappa>\<rangle>)
     \<rbrakk> \<Longrightarrow>
-    \<E> \<rightarrow> \<E> +: [
-      \<pi>;;x \<mapsto> (\<langle>e; \<rho> @: [x \<mapsto> \<lbrace>Ch \<pi> x\<rbrace>]; \<kappa>\<rangle>)
+    \<E> \<rightarrow> \<E> ++ [
+      \<pi>;;x \<mapsto> (\<langle>e; \<rho> ++ [x \<mapsto> \<lbrace>Ch \<pi> x\<rbrace>]; \<kappa>\<rangle>)
     ]
   " |
   Let_Spawn: "
     \<lbrakk> 
       leaf \<E> \<pi> ;
-      \<E> \<pi> \<diamond> \<langle>LET x = SPAWN e\<^sub>c in e; \<rho>; \<kappa>\<rangle>
+      \<E> \<pi> = Some (\<langle>LET x = SPAWN e\<^sub>c in e; \<rho>; \<kappa>\<rangle>)
     \<rbrakk> \<Longrightarrow>
-    \<E> \<rightarrow> \<E> +: [
-      \<pi>;;x \<mapsto> (\<langle>e; \<rho> @: [x \<mapsto> \<lbrace>\<rbrace>]; \<kappa>\<rangle>), 
-      \<pi>;;. \<mapsto> (\<langle>e\<^sub>c; \<rho>; [.]\<rangle>) 
+    \<E> \<rightarrow> \<E> ++ [
+      \<pi>;;x \<mapsto> (\<langle>e; \<rho> ++ [x \<mapsto> \<lbrace>\<rbrace>]; \<kappa>\<rangle>), 
+      \<pi>;;. \<mapsto> (\<langle>e\<^sub>c; \<rho>; []\<rangle>) 
     ]
   "   
 
 abbreviation concur_steps :: "state_pool \<Rightarrow> state_pool \<Rightarrow> bool" (infix "\<rightarrow>*" 55) where 
-  "x \<rightarrow>* y \<equiv> star concur_step x y"
+  "\<E> \<rightarrow>* \<E>' \<equiv> star concur_step \<E> \<E>'"
 
 end
